coupling_inv complete proof and awp_apply bug

toy.v
@@ -1,45 +1,104 @@
-From iris.algebra Require Import excl auth gmap agree gset.
-From iris.heap_lang Require Export lifting notation locations lang.
 From iris.base_logic.lib Require Export invariants.
 From iris.program_logic Require Export atomic.
 From iris.proofmode Require Import tactics.
 From iris.heap_lang Require Import proofmode notation par.
-From iris.bi.lib Require Import fractional.
-From iris.bi Require Import derived_laws_sbi.
 Set Default Proof Using "Type*".
 
-Definition write: val := 
+Definition lock : val :=
+  rec: "lockN" "x" :=
+    if: CAS "y" #false #true
+    then #()
+    else "lockN" "x".
+
+Definition unlock : val :=
+  λ: "x",
+  "y" <- #false.
+
+Definition prog : val := 
   λ: "x" "v",
-      "x" <- "v".
+  lock "x";;
+  "x" <- "v";;
+  unlock "x".
 
-Definition write2: val :=
-  λ: "x" "y" "v1" "v2",
-      write "x" "v1" ;;
-      write "y" "v2" ;; "v1".
-
-Section Give_Up_Template.
+Section Toy_Template.
   Context `{!heapG Σ} (N : namespace).
   Notation iProp := (iProp Σ).
 
-  Lemma write_spec (x: loc) v:
-         <<< ∃ d, x ↦ #d >>> write #x #v @ ⊤ <<< x ↦ #v, RET #() >>>.
-  Proof. 
-    iIntros (Φ) "AU". wp_lam. wp_let.
-    iMod "AU" as "[Hx [_ Hcl]]". iDestruct "Hx" as (d)"Hx". 
-    wp_store. iMod ("Hcl" with "Hx") as "HΦ".
-    iModIntro. done.
+
+  Definition toyN : namespace := N .@ "toy".
+
+  Definition main_inv x y (b: bool) d := (y ↦ #b ∗ if b then True else x ↦ d)%I.
+
+  Definition is_toy y := inv toyN (∃ (b:bool), y ↦ #b)%I.
+
+  Instance main_inv_timeless x y b d: Timeless (main_inv x y b d).
+  Proof.
+    rewrite /main_inv. repeat apply bi.sep_timeless; try apply _.
+    destruct b; try apply _.
   Qed.
 
-  Lemma write2_spec (x y:loc) v1 v2:
-        ((∃ d, x ↦ #d) ∗ (∃ d', y ↦ #d'))%I -∗ 
-              <<< True >>> write2 #x #y #v1 #v2 @ ⊤ <<< x ↦ #v1, RET #v1 >>>.
-  Proof. 
-    iIntros "(Hx & Hy)". iIntros (Φ) "AU". wp_lam.
-    wp_pures. wp_bind (write _ _)%E.
-    awp_apply (write_spec x v1).
-    iAaccIntro with "Hx". eauto with iFrame.
-    iIntros "H". iMod "AU" as "[Ht [_ Hcl]]".
-    iMod ("Hcl" with "H") as "HΦ".
-    iModIntro. wp_pures. wp_bind (write _ _)%E.
-    (* iDestruct "Hy" as "_". iDestruct "Ht" as "_". iDestruct "HΦ" as "_". *)
-    awp_apply (write_spec y v2).
+  Lemma lock_spec (x y: loc):
+        <<< ∀ (b: bool), y ↦ #b >>> 
+          lock #x @ ⊤ 
+        <<< y ↦ #true ∗ if b then False else True, RET #() >>>.
+  Proof.
+  Admitted.
+
+  Lemma unlock_spec (x y: loc) :
+        <<< y ↦ #true >>>
+          unlock #x @ ⊤
+        <<< y ↦ #false, RET #() >>>.
+  Proof.
+  Admitted.
+    
+  Lemma prog_spec (x y: loc) v:
+        is_toy y -∗ <<< ∀ d, x ↦ #d >>>
+                      prog #x #v @ ⊤ ∖ ↑N
+                      <<< x ↦ #v, RET #() >>>.
+  Proof.
+    iIntros "HInv". iIntros (Φ) "AU". wp_lam.
+    wp_pures. wp_bind (lock _)%E.
+    
+    (* ---------- If you don't move HInv to persistent context,
+             then following awp_apply gives an error ----------- *) 
+    iDestruct "HInv" as "#HInv".    
+    awp_apply (lock_spec x y).
+    (* --------------------------------------------------------- *)
+    
+    iInv "HInv" as ">H". iDestruct "H" as (b) "Hy".
+    iAaccIntro with "Hy". { iIntros. iModIntro.
+    iFrame. iNext. iExists b. iFrame. }
+    iIntros "(Hy & Hb)". destruct b.
+    { iExFalso. done. } iClear "Hb".
+    iModIntro. iSplitL "Hy".
+    iNext. iExists true. iFrame.
+    wp_pures. wp_bind (_ <- _)%E.
+    iMod "AU" as (d) "[Hx [_ Hclose]]".
+    wp_store. iMod ("Hclose" with "Hx") as "HΦ".
+    iModIntro. wp_pures.
+    
+    (* --------- Need to clear HΦ for the awp_appy ---------- *)
+    iClear "HΦ".
+    awp_apply (unlock_spec x y).
+    (* ------------------------------------------------------ *)
+         
+    iInv "HInv" as ">H". iDestruct "H" as (b) "Hy".
+    destruct b; last admit. 
+    iAaccIntro with "Hy". { iIntros "H". iModIntro.
+    iSplitL "H". iNext. iExists true. done. done. }
+    iIntros "Hy". iModIntro. iSplitL "Hy".
+    iNext. iExists false. done.
+    (* ------ admit HΦ ------- *)
+    admit.
+  Admitted. 
+  
+  
+  
+  
+  
+  
+  
+  
+  
+  
+     
